kore/src/Signature.v
@@ -47,3 +47,52 @@ Class Signature := {
   variables :: Variables;
   symbols :: Symbols;
 }.
+
+Module StringVariables.
+  Program Instance String_OPMLVariables {Ss : Sorts} : Variables := {|
+    evar := sort * string;
+    svar := sort * string;
+    evar_sort := fun x => fst x;
+    svar_sort := fun x => fst x;
+  |}.
+  Next Obligation.
+    unshelve econstructor.
+    * intro l.
+      pose (map (snd ∘ projT1) l) as l_mapped.
+      pose (fresh l_mapped) as new.
+      apply (existT (s, new)). simpl.
+      destruct decide. reflexivity. by simpl in n.
+    * intros. unfold fresh.
+      simpl.
+      intro.
+      apply (@infinite_is_fresh _ string_infinite (map (snd ∘ projT1) xs)).
+      unfold fresh.
+      epose proof elem_of_list_fmap_1 (snd ∘ projT1) _ _ H.
+      simpl in H0. assumption.
+    * unfold fresh.
+      intros xs ys EQ.
+      pose proof (@infinite_fresh_Permutation _ string_infinite (map (snd ∘ projT1) xs) (map (snd ∘ projT1) ys)).
+      unfold fresh in H. rewrite H. 2: reflexivity.
+      by apply Permutation_map.
+  Defined.
+  Final Obligation.
+    unshelve econstructor.
+    * intro l.
+      pose (map (snd ∘ projT1) l) as l_mapped.
+      pose (fresh l_mapped) as new.
+      apply (existT (s, new)). simpl.
+      destruct decide. reflexivity. by simpl in n.
+    * intros. unfold fresh.
+      simpl.
+      intro.
+      apply (@infinite_is_fresh _ string_infinite (map (snd ∘ projT1) xs)).
+      unfold fresh.
+      epose proof elem_of_list_fmap_1 (snd ∘ projT1) _ _ H.
+      simpl in H0. assumption.
+    * unfold fresh.
+      intros xs ys EQ.
+      pose proof (@infinite_fresh_Permutation _ string_infinite (map (snd ∘ projT1) xs) (map (snd ∘ projT1) ys)).
+      unfold fresh in H. rewrite H. 2: reflexivity.
+      by apply Permutation_map.
+  Defined.
+End StringVariables.
