kore/src/Substitution.v
@@ -1,0 +1,3 @@
+From Kore Require Export Syntax.
+
+Import Kore.Syntax.Notations.
